\begin{frame}[plain]{Merger Resolution}
    \begin{figure}
        \centering
        \scalebox{0.7}{
            \begin{tikzpicture}[minimum size=58pt,scale=0.45, every node/.style={scale=0.45, font=\LARGE}, thick]
                \input{images/conservation/hypotheses_original.tex}
            \end{tikzpicture}
        }
        \caption{Original hypotheses graph.}
        \label{fig:conservation-hyp-inferred}
    \end{figure}
\end{frame}

\begin{frame}[plain]{Merger Resolution}
    \begin{figure}
        \centering
        \scalebox{0.7}{
            \begin{tikzpicture}[minimum size=58pt,scale=0.45, every node/.style={scale=0.45, font=\LARGE}, thick]
                \input{images/conservation/hypotheses_after_inference.tex}
            \end{tikzpicture}
        }
        \caption{Inferred configuration of the hypotheses graph.}
        \label{fig:conservation-hyp-inferred}
    \end{figure}
\end{frame}

\begin{frame}[plain]{Merger Resolution}
    \begin{figure}
        \centering
        \scalebox{0.7}{
            \begin{tikzpicture}[minimum size=58pt,scale=0.45, every node/.style={scale=0.45, font=\LARGE}, thick]
                \input{images/conservation/hypotheses_subset.tex}
            \end{tikzpicture}
        }
        \caption{Subset of the hypotheses graph that contains all merged objects.}
        \label{fig:conservation-hyp-inferred}
    \end{figure}
\end{frame}

\begin{frame}[plain]{Merger Resolution}
    \begin{figure}
        \centering
        \scalebox{0.7}{
            \begin{tikzpicture}[minimum size=58pt,scale=0.45, every node/.style={scale=0.45, font=\LARGE}, thick]
                \input{images/conservation/hypotheses_subset_inferred.tex}
            \end{tikzpicture}
        }
        \caption{Inferred configuration of the subset.}
        \label{fig:conservation-hyp-inferred}
    \end{figure}
\end{frame}


\begin{frame}[plain]{Merger Resolution - Divisions}
    \begin{figure}
        \centering
        \scalebox{0.8}{
            \begin{tikzpicture}[minimum size=58pt,scale=0.45, every node/.style={scale=0.45, font=\LARGE}, thick]
                \input{images/conservation/division_detected.tex}
            \end{tikzpicture}
        }
    \end{figure}
\end{frame}

\begin{frame}[plain]{Merger Resolution - Divisions}
    \begin{figure}
        \centering
        \scalebox{0.8}{
            \begin{tikzpicture}[minimum size=58pt,scale=0.45, every node/.style={scale=0.45, font=\LARGE}, thick]
                \input{images/conservation/division_duplicated.tex}
            \end{tikzpicture}
        }
    \end{figure}
\end{frame}

\begin{frame}[plain]{Merger Resolution - Divisions}
    \begin{figure}
        \centering
        \scalebox{0.8}{
            \begin{tikzpicture}[minimum size=58pt,scale=0.45, every node/.style={scale=0.45, font=\LARGE}, thick]
                \input{images/conservation/division_inferred.tex}
            \end{tikzpicture}
        }
    \end{figure}
\end{frame}


\begin{frame}[plain]
    \frametitle{Factors - Detection/Conflict}
    \begin{align*}
        \psi_{\text{det}}(\mathcal{K}_{i\nu}^t, \xi_{i\nu}^t) &=
        e^{-E_{\text{det}}(\mathcal{K}_{i\nu}^t, \xi_{i\nu}^t)} \\
        E_{\text{det}}(\mathcal{K}_{i\nu}^t, \xi_{i\nu}^t)&=
        \begin{cases}
            A(\mathcal{K}_{i\nu}^t, \xi_{i\nu}^t), &\text{if} \sum_{X \in \mathcal{K}_{i\nu}^t} X = 1 \\ 
            B(\mathcal{K}_{i\nu}^t, \xi_{i\nu}^t), &\text{if} \sum_{X \in \mathcal{K}_{i\nu}^t} X = 0 \\ 
            \infty, &\text{otherwise}
        \end{cases}
    \end{align*}
    with
    \begin{align*}
        A(\mathcal{K}_{i\nu}^t, \xi_{i\nu}^t) &=-w_{\text{det}} \sum_{X_{i\alpha}^t \in \mathcal{K}_{i\nu}^t}
        \mathds{1} \left(X_{i\alpha}^t =
            1\right)\log\left(\hat{P}(X_{i\alpha}^t=1|f_{i\alpha}^t)\right),
        \\
        B(\mathcal{K}_{i\nu}^t, \xi_{i\nu}^t) &= -w_{\text{det}} \max_{X_{i\alpha}^t\in\mathcal{K}_{i\nu}^t}
        \log\left(\hat{P}(X_{i\alpha}^t = 0|f_{i\alpha}^t)\right) + c_{\text{opp}}
    \end{align*}
\end{frame}


\begin{frame}[plain]
    \frametitle{Factors - Count}
    \begin{align*}
        \psi_{\text{count}}(\{X_{i\alpha}^t\}_{\alpha \in
            I_i^t},f_{i}^t)&=e^{-E_{\text{count}}(\{(X_{i\alpha}^t,f_{i\alpha}^t)\}_{\alpha \in I_i^t})}, \\
        E_{\text{count}}(\{X_{i\alpha}^t\}_{\alpha \in I_i^t},f_{i}^t) &=
        -w_{\text{count}}\log\left(\hat{P}_{\text{count}}\left(\sum_{X \in \{X_{i\alpha}^t\}_{\alpha \in
                        I_i^t}}X=k|f_i^t\right)\right)
    \end{align*}
\end{frame}


\begin{frame}[plain]
    \frametitle{Factors - Outgoing}
    \begin{align*}
        \psi_{\mathrm{out}}(X_{i\alpha}^t, \mathcal{Y}_{i\alpha\rightarrow}^{t}, f_{i\alpha}^t,
        \Xi_{i\alpha\rightarrow}^{t}) &=
        e^{-E_{\mathrm{out}}(X_{i\alpha}^t, \mathcal{Y}_{i\alpha\rightarrow}^{t}, f_{i\alpha}^t, \Xi_{i\alpha\rightarrow}^{t})} \\
        E_{\mathrm{out}}(X_{i\alpha}^t, \mathcal{Y}_{i\alpha\rightarrow}^{t}, f_{i\alpha}^t,
        \Xi_{i\alpha\rightarrow}^{t}) &= E_{\text{dis}}(X_{i\alpha}^t,
        \mathcal{Y}_{i\alpha\rightarrow}^{t}) \\ \nonumber
        &+ E_{\text{move}}(X_{i\alpha}^t, \mathcal{Y}_{i\alpha\rightarrow}^{t}, f_{i\alpha}^t,
        \Xi_{i\alpha\rightarrow}^{t}) \\ \nonumber
        &+ E_{\text{div}}(X_{i\alpha}^t, \mathcal{Y}_{i\alpha\rightarrow}^{t}, f_{i\alpha}^t,
        \Xi_{i\alpha\rightarrow}^{t}) \\ \nonumber
        &+ E_{\text{out,for}}(X_{i\alpha}^t, \mathcal{Y}_{i\alpha\rightarrow}^{t})
    \end{align*}
\end{frame}


\begin{frame}[plain]
    \frametitle{Factors - Outgoing: Disappearance}
    \begin{align*}
        E_{\mathrm{dis}}(X_{i\alpha}^t,  \mathcal{Y}_{i\alpha\rightarrow}^{t}) &=
        \begin{cases}
            C(X_{i\alpha}^t, \mathcal{Y}_{i\alpha\rightarrow}^{t}), & X_{i\alpha}^t = 1 \wedge
            \sum_{Y\in\mathcal{Y}_{i\alpha\rightarrow}^{t}}Y = 0 \\
            0, & \text{otherwise}
        \end{cases} \\
        C(X_{i\alpha}^t, \mathcal{Y}_{i\alpha\rightarrow}^{t}) &= w_{\mathrm{dis}} \cdot
        \frac{|X_{i\alpha}^t|} {\max_{\kappa \in I_i^t}|X_{i\kappa}^t|} \\
        &+ \max\left(E_{\text{move}}(X_{i\alpha}^t, \mathcal{Y}_{i\alpha\rightarrow}^{t}), E_{\text{div}}(X_{i\alpha}^t, \mathcal{Y}_{i\alpha\rightarrow}^{t})\right)
    \end{align*}
\end{frame}


\begin{frame}[plain]
    \frametitle{Factors - Outgoing: Division}
    \begin{align*}
        E_{\mathrm{div}}&(X_{i\alpha}^t, \mathcal{Y}_{i\alpha\rightarrow}^{t}, f_{i\alpha}^t,
        \Xi_{i\alpha\rightarrow}^{t}) \\ \nonumber
        &=-w_{\mathrm{div}} \cdot \frac{|X_{i\alpha}^t|} {\max_{\kappa \in I_i^t}|X_{i\kappa}^t|} \\ \nonumber
        &\phantom{=}\times
        \begin{cases}
            \log (F(X_{i\alpha}^t, \mathcal{Y}_{i\alpha\rightarrow}^{t}, f_{i\alpha}^t,
            \Xi_{i\alpha\rightarrow}^{t})), & \sum_{Y\in\mathcal{Y}_{i\alpha\rightarrow}^{t}}Y=2 \\
            0, &\text{otherwise}
        \end{cases}
    \end{align*}
    \begin{alignat}{3}
        \nonumber
        F&(X_{i\alpha}^t, \mathcal{Y}_{i\alpha\rightarrow}^{t}, f_{i\alpha}^t,
        \Xi_{i\alpha\rightarrow}^{t}) \\ \nonumber
        &=\mathlarger{\mathlarger{\sum}}_{\mathsmaller{\substack{Y_{i\alpha,j_1\kappa_1}^t \in
                    \mathcal{Y}_{i\alpha\rightarrow}^{t}, \\ \nonumber
                    Y_{i\alpha,j_2\kappa_2}^t \in \mathcal{Y}_{i\alpha\rightarrow}^{t},\\ \nonumber
                    Y_{i\alpha,j_2\kappa_2}^t \ne Y_{i\alpha,j_1\kappa_1}^t}}}
        \Bigg(\hat{P}_{\mathrm{div}}\left(Y_{i\alpha,j_1\kappa_1}^t=1,Y_{i\alpha,j_2\kappa_2^t}=1|f_{i\alpha}^t,f_{j_1\kappa_1}^{t+1},f_{j_2\kappa_2}^{t+1}\right)
        \\[-35pt] \nonumber
        &\phantom{=}\quad\quad\quad\quad\quad\quad\quad\;\;\;\;\times\mathds{1}(Y_{i\alpha,j_1\kappa_1}^t=1)\mathds{1}(Y_{i\alpha,j_2\kappa_2}^t=1)\Bigg)
    \end{alignat}
\end{frame}


\begin{frame}[plain]
    \frametitle{Factors - Outgoing: Move}
    \begin{align*}
        E_{\text{move}}&(X_{i\alpha}^t, \mathcal{Y}_{i\alpha\rightarrow}^{t}, f_{i\alpha}^t,
        \Xi_{i\alpha\rightarrow}^{t}) \\ \nonumber
        &=-w_{\text{move}} \cdot \frac{|X_{i\alpha}^t|}{\max_{\kappa \in I_i^t}|X_{i\kappa}^t|} \\
        \nonumber
        &\phantom{=}\times
        \begin{cases}
            \log (G(X_{i\alpha}^t, \mathcal{Y}_{i\alpha\rightarrow}^{t}, f_{i\alpha}^t,
            \Xi_{i\alpha\rightarrow}^{t})), & \sum_{Y\in\mathcal{Y}_{i\alpha\rightarrow}^{t}}Y=1 \\
            0, &\text{otherwise},
        \end{cases}
    \end{align*}
    \begin{align*}
        G&(X_{i\alpha}^t, \mathcal{Y}_{i\alpha\rightarrow}^{t}, f_{i\alpha}^t,
        \Xi_{i\alpha\rightarrow}^{t}) \\ \nonumber
        &=\mathlarger{\mathlarger{\sum}}_{\mathsmaller{\substack{Y_{i\alpha,j\kappa}^t \in \mathcal{Y}_{i\alpha\rightarrow}^{t}}}}
        \Bigg(\hat{P}_{\mathrm{move}}\left(Y_{i\alpha,j\kappa}^t=1|f_{i\alpha}^t,f_{j\kappa}^{t+1}\right)
        \cdot\mathds{1}(Y_{i\alpha,j\kappa}^t=1)\Bigg)
    \end{align*}
\end{frame}


\begin{frame}[plain]
    \frametitle{Factors - Outgoing: Forbidden}
    \begin{align*}
        E_{\text{out,for}}(X_{i\alpha}^t, \mathcal{Y}_{i\alpha\rightarrow}^{t})=
        \begin{cases}
            \infty, & \sum_{Y \in \mathcal{Y}_{i\alpha\rightarrow}^{t}}Y > 2 \\
            \infty, & \sum_{Y \in \mathcal{Y}_{i\alpha\rightarrow}^{t}}Y > 0 \wedge X_{i\alpha}^t = 0 \\
            0, \text{otherwise}
        \end{cases}
    \end{align*}
\end{frame}


\begin{frame}[plain]
    \frametitle{Factors - Incoming}
    \begin{align*}
        \psi_{\mathrm{in}}(X_{j\beta}^{t+1}, \mathcal{Y}_{\rightarrow j\beta}^{t})
        &= e^{-E_{\text{in}}(X_{j\beta}^{t+1},  \mathcal{Y}_{\rightarrow j\beta}^{t})} \\
        E_\text{in}(X_{j\beta}^{t+1},  \mathcal{Y}_{\rightarrow j\beta}^{t}) &= E_{\text{app}}(X_{j\beta}^{t+1},
        \mathcal{Y}_{\rightarrow j\beta}^{t}) \\
        &+ E_{\text{in,for}}(X_{j\beta}^{t+1},  \mathcal{Y}_{\rightarrow j\beta}^{t})
    \end{align*}
\end{frame}


\begin{frame}[plain]
    \frametitle{Factors - Outgoing: Appearance}
    \begin{align*}
        E_{\text{app}}&(X_{j\beta}^{t+1}, \mathcal{Y}_{\rightarrow, j\beta}^t) \\ \nonumber
        &=
        \begin{cases}
            \frac{|X_{j\beta}^{t+1}|} {\max_{\kappa \in I_j^{t+1}}|X_{j\kappa}^{t+1}|} \cdot w_{\mathrm{app}}, & X_{j\beta}^{t+1} = 1 \wedge \sum_{Y\in\mathcal{Y}_{\rightarrow, j\beta}^t}Y = 0 \\
            0, & \mathrm{otherwise}
        \end{cases}    
    \end{align*}
\end{frame}


\begin{frame}[plain]
    \frametitle{Factors - Incoming: Forbidden}
    \begin{align*}
        E_{\text{in,for}}(X_{j\beta}^{t+1},  \mathcal{Y}_{\rightarrow j\beta}^{t})=
        \begin{cases}
        \infty, & \sum_{Y \in \mathcal{Y}_{\rightarrow j\beta}^{t}}Y >
        1 \\
        \infty, & \sum_{Y \in \mathcal{Y}_{\rightarrow j\beta}^{t}}Y > 0 \wedge X_{j\beta}^{t+1} =
        0 \\
        0, & \text{otherwise}
        \end{cases}
    \end{align*}
\end{frame}


%%% Local Variables: 
%%% mode: latex
%%% TeX-master: "../main"
%%% End: 
